src/StackCompCombined.v
@@ -15,356 +15,48 @@ Require
     StackFlatterComp2
 .
 
-Definition compile_cont (cu : Switched2.prog_type) : res StackCont.prog_type :=
-  OK cu
-  @@@ StackMachComp.compile_cu
-  @@ StackContComp.compile_cu.
-
-Section FSIMcont.
-
-  Variable a : Switched2.prog_type.
-  Variable b : StackCont.prog_type.
-  Hypothesis TRANSF : compile_cont a = OK b.
-
-  Lemma compile_cont_succ :
-    { c | StackMachComp.compile_cu a = Some c }.
-  Proof.
-    unfold compile_cont in TRANSF. break_result_chain. eauto.
-  Qed.
-  
-  Definition fsim_cont : Semantics.forward_simulation (Switched2.semantics a) (StackCont.semantics b).
-    destruct compile_cont_succ.
-    eapply Semantics.compose_forward_simulation;
-      try eapply StackMachComp.fsim; eauto;
-      try eapply StackContComp.fsim; eauto.
-    unfold compile_cont in *; break_result_chain.
-    congruence.
-  Defined.
-
-  Lemma fsim_cont_match_val :
-    forall x y,
-      Semantics.fsim_match_val _ _ fsim_cont x y <-> eq x y.
-  Proof.
-    intros. unfold fsim_cont.
-    destruct compile_cont_succ.
-    erewrite Semantics.fsim_match_val_compose. repeat instantiate (1 := eq).
-    split; intros; repeat break_exists; repeat eexists; repeat break_and; eauto; try congruence.
-    erewrite StackMachComp.match_val_eq.
-    intros; split; intros; congruence.
-    erewrite StackContComp.match_val_eq.
-    intros; split; intros; congruence.
-  Qed.    
-
-End FSIMcont.
-
-Definition compile_cont2 (cu : Switched2.prog_type) : res StackCont2.prog_type :=
-  OK cu
-  @@@ compile_cont
-  @@ StackContComp2.compile_cu.
-
-Section FSIMcont2.
-
-  Variable a : Switched2.prog_type.
-  Variable b : StackCont2.prog_type.
-  Hypothesis TRANSF : compile_cont2 a = OK b.
-
-  Lemma compile_cont2_succ :
-    { c | compile_cont a = Some c }.
-  Proof.
-    unfold compile_cont2 in TRANSF. break_result_chain. eauto.
-  Qed.
-  
-  Definition fsim_cont2 : Semantics.forward_simulation (Switched2.semantics a) (StackCont2.semantics b).
-    destruct compile_cont2_succ.
-    eapply Semantics.compose_forward_simulation;
-      try eapply fsim_cont; eauto;
-      try eapply StackContComp2.fsim; eauto.
-    unfold compile_cont2 in *; break_result_chain.
-    unfold option_to_res in *. congruence.
-  Defined.
-
-  Lemma fsim_cont2_match_val :
-    forall x y,
-      Semantics.fsim_match_val _ _ fsim_cont2 x y <-> eq x y.
-  Proof.
-    intros. unfold fsim_cont2.
-    destruct compile_cont2_succ.
-    erewrite Semantics.fsim_match_val_compose. repeat instantiate (1 := eq).
-    split; intros; repeat break_exists; repeat eexists; repeat break_and; eauto; try congruence.
-    intros. erewrite fsim_cont_match_val.
-    intros; split; intros; congruence.
-    erewrite StackContComp2.match_val_eq.
-    intros; split; intros; congruence.
-  Qed.    
-
-End FSIMcont2.
-
-Definition compile_cont3 (cu : Switched2.prog_type) : res StackCont3.prog_type :=
-  OK cu
-  @@@ compile_cont2
-  @@ StackContComp3.compile_cu.
-
-Section FSIMcont3.
-
-  Variable a : Switched2.prog_type.
-  Variable b : StackCont3.prog_type.
-  Hypothesis TRANSF : compile_cont3 a = OK b.
-
-  Lemma compile_cont3_succ :
-    { c | compile_cont2 a = Some c }.
-  Proof.
-    unfold compile_cont3 in TRANSF. break_result_chain. eauto.
-  Qed.
-  
-  Definition fsim_cont3 : Semantics.forward_simulation (Switched2.semantics a) (StackCont3.semantics b).
-    destruct compile_cont3_succ.
-    eapply Semantics.compose_forward_simulation;
-      try eapply fsim_cont2; eauto;
-        try eapply StackContComp3.fsim; eauto.
-    unfold compile_cont3 in *; break_result_chain.
-    unfold option_to_res in *. congruence.
-  Defined.
-
-  Lemma fsim_cont3_match_val :
-    forall x y,
-      Semantics.fsim_match_val _ _ fsim_cont3 x y <-> eq x y.
-  Proof.
-    intros. unfold fsim_cont3.
-    destruct compile_cont3_succ.
-    erewrite Semantics.fsim_match_val_compose. repeat instantiate (1 := eq).
-    split; intros; repeat break_exists; repeat eexists; repeat break_and; eauto; try congruence.
-    intros. erewrite fsim_cont2_match_val.
-    intros; split; intros; congruence.
-    erewrite StackContComp3.match_val_eq.
-    intros; split; intros; congruence.
-  Qed.    
-
-End FSIMcont3.
-
-Definition compile_flat (cu : Switched2.prog_type) : res StackFlat.prog_type :=
-  OK cu
-  @@@ compile_cont3
-  @@ StackFlatComp.compile_cu.
-
-Section FSIMflat.
-
-  Variable a : Switched2.prog_type.
-  Variable b : StackFlat.prog_type.
-  Hypothesis TRANSF : compile_flat a = OK b.
-
-  Lemma compile_flat_succ :
-    { c | compile_cont3 a = OK c }.
-  Proof.
-    unfold compile_flat in TRANSF. break_result_chain. eauto.
-  Qed.
-  
-  Definition fsim_flat : Semantics.forward_simulation (Switched2.semantics a) (StackFlat.semantics b).
-    destruct compile_flat_succ.
-    eapply Semantics.compose_forward_simulation;
-      try eapply fsim_cont3; eauto;
-        try eapply StackFlatComp.fsim; eauto.
-    unfold compile_flat in *; break_result_chain.
-    unfold option_to_res in *. congruence.
-  Defined.
-
-  Lemma fsim_flat_match_val :
-    forall x y,
-      Semantics.fsim_match_val _ _ fsim_flat x y <-> eq x y.
-  Proof.
-    intros. unfold fsim_flat.
-    destruct compile_flat_succ.
-    erewrite Semantics.fsim_match_val_compose. repeat instantiate (1 := eq).
-    split; intros; repeat break_exists; repeat eexists; repeat break_and; eauto; try congruence.
-    intros. erewrite fsim_cont3_match_val.
-    intros; split; intros; congruence.
-    erewrite StackFlatComp.match_val_eq.
-    intros; split; intros; congruence.
-  Qed.    
-
-End FSIMflat.
-
-Definition compile_flatter (cu : Switched2.prog_type) : res StackFlatter.prog_type :=
-  OK cu
-  @@@ compile_flat
-  @@ StackFlatterComp.compile_cu.
-
-Section FSIMflatter.
-
-  Variable a : Switched2.prog_type.
-  Variable b : StackFlatter.prog_type.
-  Hypothesis TRANSF : compile_flatter a = OK b.
-
-  Lemma compile_flatter_succ :
-    { c | compile_flat a = OK c }.
-  Proof.
-    unfold compile_flatter in TRANSF. break_result_chain. eauto.
-  Qed.
-  
-  Definition fsim_flatter : Semantics.forward_simulation (Switched2.semantics a) (StackFlatter.semantics b).
-    destruct compile_flatter_succ.
-    eapply Semantics.compose_forward_simulation;
-      try eapply fsim_flat; eauto;
-        try eapply StackFlatterComp.fsim; eauto.
-    unfold compile_flatter in *; break_result_chain.
-    unfold option_to_res in *. congruence.
-  Defined.
-
-  Lemma fsim_flatter_match_val :
-    forall x y,
-      Semantics.fsim_match_val _ _ fsim_flatter x y <-> eq x y.
-  Proof.
-    intros. unfold fsim_flatter.
-    destruct compile_flatter_succ.
-    erewrite Semantics.fsim_match_val_compose. repeat instantiate (1 := eq).
-    split; intros; repeat break_exists; repeat eexists; repeat break_and; eauto; try congruence.
-    intros. erewrite fsim_flat_match_val.
-    intros; split; intros; congruence.
-    erewrite StackFlatterComp.match_val_eq.
-    intros; split; intros; congruence.
-  Qed.    
-
-End FSIMflatter.
-
-Definition compile_flatter2 (cu : Switched2.prog_type) : res StackFlatter2.prog_type :=
-  OK cu
-  @@@ compile_flatter
-  @@ StackFlatterComp2.compile_cu.
-
-Section FSIMflatter2.
-
-  Variable a : Switched2.prog_type.
-  Variable b : StackFlatter2.prog_type.
-  Hypothesis TRANSF : compile_flatter2 a = OK b.
-
-  Lemma compile_flatter2_succ :
-    { c | compile_flatter a = OK c }.
-  Proof.
-    unfold compile_flatter2 in TRANSF. break_result_chain. eauto.
-  Qed.
-  
-  Definition fsim_flatter2 : Semantics.forward_simulation (Switched2.semantics a) (StackFlatter2.semantics b).
-    destruct compile_flatter2_succ.
-    eapply Semantics.compose_forward_simulation;
-      try eapply fsim_flatter; eauto;
-        try eapply StackFlatterComp2.fsim; eauto.
-    unfold compile_flatter2 in *; break_result_chain.
-    unfold option_to_res in *. congruence.
-  Defined.
-
-  Lemma fsim_flatter2_match_val :
-    forall x y,
-      Semantics.fsim_match_val _ _ fsim_flatter2 x y <-> eq x y.
-  Proof.
-    intros. unfold fsim_flatter2.
-    destruct compile_flatter2_succ.
-    erewrite Semantics.fsim_match_val_compose. repeat instantiate (1 := eq).
-    split; intros; repeat break_exists; repeat eexists; repeat break_and; eauto; try congruence.
-    intros. erewrite fsim_flatter_match_val.
-    intros; split; intros; congruence.
-    erewrite StackFlatterComp2.match_val_eq.
-    intros; split; intros; congruence.
-  Qed.    
-
-End FSIMflatter2.
-
-
-
-
 
 Module A := Switched2.
 Module B := StackFlatter2.
 
-Definition compile_cu (cu : A.env * list metadata) : res (B.env * list metadata) :=
-  compile_flatter2 cu.
+Definition compile_cu (cu : A.prog_type) : res B.prog_type :=
+        OK cu
+    @@@ StackMachComp.compile_cu
+    @@  StackContComp.compile_cu
+    @@  StackContComp2.compile_cu
+    @@  StackContComp3.compile_cu
+    @@  StackFlatComp.compile_cu
+    @@  StackFlatterComp.compile_cu
+    @@  StackFlatterComp2.compile_cu
+.
+
 
 Section Preservation.
 
-  Variable prog : A.prog_type.
-  Variable tprog : B.prog_type.
+Variable aprog : A.prog_type.
+Variable bprog : B.prog_type.
 
-  Hypothesis TRANSF : compile_cu prog = OK tprog.
+Hypothesis Hcomp : compile_cu aprog = OK bprog.
 
-  Definition fsim : Semantics.forward_simulation (A.semantics prog) (B.semantics tprog).
-    eapply fsim_flatter2. assumption.
-  Defined.
+Definition fsim : Semantics.forward_simulation (A.semantics aprog) (B.semantics bprog).
+  unfold compile_cu in Hcomp.
+  break_result_chain.
 
-  Lemma match_val_eq :
-    forall x y,
-      Semantics.fsim_match_val _ _ fsim x y <-> eq x y.
-  Proof.
-    eapply fsim_flatter2_match_val.
-  Qed.
+  eapply Semantics.compose_forward_simulation. eauto using StackMachComp.fsim.
+  eapply Semantics.compose_forward_simulation. eauto using StackContComp.fsim.
+  eapply Semantics.compose_forward_simulation. eauto using StackContComp2.fsim.
+  eapply Semantics.compose_forward_simulation. eauto using StackContComp3.fsim.
+  eapply Semantics.compose_forward_simulation. eauto using StackFlatComp.fsim.
+  eapply Semantics.compose_forward_simulation. eauto using StackFlatterComp.fsim.
+  eauto using StackFlatterComp2.fsim.
+Qed.
+
+Lemma fsim_match_val :
+  forall x y,
+    Semantics.fsim_match_val _ _ fsim x y <-> x = y.
+Proof.
+  intros. erewrite (Semantics.fsim_match_val_canon _ _ fsim).
+  simpl. tauto.
+Qed.
 
 End Preservation.
-
-
-
-Inductive I : A.state -> B.state -> Prop :=
-| ICombined : forall s00 s01 s02 s03 s04 s05 s06 s07,
-        StackMachComp.I         s00 s01 ->
-        StackContComp.I         s01 s02 ->
-        StackContComp2.I        s02 s03 ->
-        StackContComp3.I        s03 s04 ->
-        StackFlatComp.I         s04 s05 ->
-        StackFlatterComp.I      s05 s06 ->
-        StackFlatterComp2.I     s06 s07 ->
-        I s00 s07.
-
-Inductive I_func : A.expr -> list B.insn -> Prop :=
-| IFuncCombined : forall f00 f01 f02 f03 f04 f05 f06 f07,
-        StackMachComp.I_expr []             f00 f01 ->
-        Forall2 StackContComp.I_insn        f01 f02 ->
-        Forall2 StackContComp2.I_insn       f02 f03 ->
-        Forall2 StackContComp3.I_insn       f03 f04 ->
-        Forall2 StackFlatComp.I_insn        f04 f05 ->
-        StackFlatterComp.I_insns            f05 f06 ->
-        StackFlatterComp2.I_insns           f06 f07 ->
-        I_func f00 f07.
-
-
-Lemma chain_I_env :
-    forall e00 e01 e02 e03 e04 e05 e06 e07,
-        Forall2 (StackMachComp.I_expr [])           e00 e01 ->
-        Forall2 (Forall2 StackContComp.I_insn)      e01 e02 ->
-        Forall2 (Forall2 StackContComp2.I_insn)     e02 e03 ->
-        Forall2 (Forall2 StackContComp3.I_insn)     e03 e04 ->
-        Forall2 (Forall2 StackFlatComp.I_insn)      e04 e05 ->
-        Forall2 (StackFlatterComp.I_insns)          e05 e06 ->
-        Forall2 (StackFlatterComp2.I_insns)         e06 e07 ->
-        Forall2 I_func e00 e07.
-intros.
-list_magic_on (e00, (e01, (e02, (e03, (e04, (e05, (e06, (e07, tt)))))))).
-eapply IFuncCombined; eassumption.
-Qed.
-
-
-
-Theorem compile_I_func : forall a ameta b bmeta,
-    compile_cu (a, ameta) = OK (b, bmeta) ->
-    Forall2 I_func a b.
-intros0 Hcomp. unfold compile_cu in *.
-
-unfold compile_flatter2 in *.
-unfold compile_flatter in *.
-unfold compile_flat in *.
-unfold compile_cont3 in *.
-unfold compile_cont2 in *.
-unfold compile_cont in *.
-remember (a, ameta) as aprog.
-break_result_chain.
-subst aprog.  repeat on (_ * _)%type, fun x => destruct x.
-
-on _, eapply_lem StackMachComp.compile_cu_I_env.
-on _, eapply_lem StackContComp.compile_cu_I_env.
-on _, eapply_lem StackContComp2.compile_cu_I_env.
-on _, eapply_lem StackContComp3.compile_cu_I_env.
-on _, eapply_lem StackFlatComp.compile_cu_I_env.
-on _, eapply_lem StackFlatterComp.compile_cu_I_env.
-on _, eapply_lem StackFlatterComp2.compile_cu_I_env.
-
-eapply chain_I_env; eassumption.
-Qed.
-
-
-
-
