src/ElimFuncComp4.v
@@ -1213,22 +1213,12 @@ Section Preservation.
       econstructor; eauto.
       + unfold fst, snd in *. eauto using compile_cu_public_value'.
 
+    - simpl. eauto.
+    - simpl. intros. tauto.
+
     - intros0 Astep. intros0 II.
       eapply splus_semantics_sim, I'_sim; eauto.
 
-    Defined.
-
-    Lemma match_val_eq :
-      Semantics.fsim_match_val _ _ fsim = eq.
-    Proof.
-      unfold fsim. simpl.
-      unfold Semantics.fsim_match_val.
-      break_match. repeat (break_match_hyp; try congruence).
-      try unfold forward_simulation_step in *.
-      try unfold forward_simulation_plus in *.
-      try unfold forward_simulation_star in *.
-      try unfold forward_simulation_star_wf in *.
-      inv Heqf. reflexivity.
     Qed.
 
 End Preservation.
