src/ElimFuncCompCombined.v
@@ -1,0 +1,69 @@
+Require Import compcert.driver.Compiler compcert.common.Errors.
+Require Import Common Monads.
+Require CompilationUnit.
+Require Import Metadata.
+Require Import CompilerUtil.
+Require MatchValues.
+
+Require Untyped8 Switched2.
+Require
+    TaggedComp
+    ElimFuncComp1
+    ElimFuncComp2
+    ElimFuncComp3
+    ElimFuncComp4
+    SelfCloseComp
+    MkCloseSelfOpt
+    SwitchedComp1
+    SwitchedComp2
+.
+
+
+Module A := Untyped8.
+Module B := Switched2.
+
+Definition compile_cu (cu : A.prog_type) : res B.prog_type :=
+        OK cu
+    @@@ TaggedComp.compile_cu
+    @@@ ElimFuncComp1.compile_cu
+    @@@ ElimFuncComp2.compile_cu
+    @@  ElimFuncComp3.compile_cu
+    @@@ ElimFuncComp4.compile_cu
+    @@  SelfCloseComp.compile_cu
+    @@@ MkCloseSelfOpt.compile_cu
+    @@@ SwitchedComp1.compile_cu
+    @@@ SwitchedComp2.compile_cu
+.
+
+
+Section Preservation.
+
+Variable aprog : A.prog_type.
+Variable bprog : B.prog_type.
+
+Hypothesis Hcomp : compile_cu aprog = OK bprog.
+
+Definition fsim : Semantics.forward_simulation (A.semantics aprog) (B.semantics bprog).
+  unfold compile_cu in Hcomp.
+  break_result_chain.
+
+  eapply Semantics.compose_forward_simulation. eauto using TaggedComp.fsim.
+  eapply Semantics.compose_forward_simulation. eauto using ElimFuncComp1.fsim.
+  eapply Semantics.compose_forward_simulation. eauto using ElimFuncComp2.fsim.
+  eapply Semantics.compose_forward_simulation. eauto using ElimFuncComp3.fsim.
+  eapply Semantics.compose_forward_simulation. eauto using ElimFuncComp4.fsim.
+  eapply Semantics.compose_forward_simulation. eauto using SelfCloseComp.fsim.
+  eapply Semantics.compose_forward_simulation. eauto using MkCloseSelfOpt.fsim.
+  eapply Semantics.compose_forward_simulation. eauto using SwitchedComp1.fsim.
+  eauto using SwitchedComp2.fsim.
+Qed.
+
+Lemma fsim_match_val :
+  forall x y,
+    Semantics.fsim_match_val _ _ fsim x y <-> MatchValues.mv_higher x y.
+Proof.
+  intros. erewrite (Semantics.fsim_match_val_canon _ _ fsim).
+  simpl. tauto.
+Qed.
+
+End Preservation.
